

## Hermitian of Matrix:

The hermitian of matrix  $A$  is denoted by  $A^H$  ( $A^*$ ) and is defined as conjugate transpose of  $A$  i.e.  $A^H = \overline{(A^T)} = (\bar{A})'$

## Hermitian Matrix:

A square matrix  $A$  is said to be Hermitian Matrix if  $A = A^H$

## Skew-Hermitian Matrix:

The square matrix  $A$  is said to be skew-Hermitian Matrix if  $A = -A^H$

"Every square matrix can be uniquely expressed as a sum of a Hermitian Matrix and a Skew-Hermitian Matrix"

{ Hint ① Replace ( ) by ( ) }  
②  $(A^\theta)^\theta = A$

### Unitary Matrix

A square matrix  $A$  is said to be unitary matrix if  $AA^\theta = A^\theta A = I$

Remark: If  $A$  is unitary matrix then  $A^{-1} = A^\theta$

Ex. Prove that  $A = \frac{1}{2} \begin{bmatrix} 1+i & -1+i \\ 1+i & 1-i \end{bmatrix}$

is unitary and hence find  $A^{-1}$

Sol<sup>n</sup>: Let  $A = \frac{1}{2} \begin{bmatrix} 1+i & -1+i \\ 1+i & 1-i \end{bmatrix}$

$$A^\theta = \frac{1}{2} \begin{bmatrix} 1+i & 1+i \\ -1+i & 1-i \end{bmatrix}$$

$$A^\theta = \overline{(A')} = \frac{1}{2} \begin{bmatrix} 1-i & 1-i \\ -1-i & 1+i \end{bmatrix}$$

we have

$$AA^0 = \frac{1}{2} \begin{bmatrix} 1+i & -1+i \\ 1+i & 1-i \end{bmatrix} \frac{1}{2} \begin{bmatrix} 1-i & 1-i \\ -1-i & 1+i \end{bmatrix} \left\{ \begin{aligned} (x+iy)(x-iy) &= x^2+y^2 \\ z^2 &= -1 \end{aligned} \right\}$$

$$= \frac{1}{4} \begin{bmatrix} 1+i & -1+i \\ 1+i & 1-i \end{bmatrix} \begin{bmatrix} 1-i & 1-i \\ -1-i & 1+i \end{bmatrix}$$

$$= \frac{1}{4} \begin{bmatrix} (1+i)(1-i) + (-1+i)(-1-i) & (1+i)(1-i) + (-1+i)(1+i) \\ (1+i)(1-i) + (1-i)(-1-i) & (1+i)(1-i) + (1-i)(1+i) \end{bmatrix}$$

$$= \frac{1}{4} \begin{bmatrix} 1+1+1+1 & 1+1-i-i^2+i^2-1-i \\ 1+1-1-i+i+i^2 & 1+1+1+1 \end{bmatrix}$$

$$= \frac{1}{4} \begin{bmatrix} 4 & 0 \\ 0 & 4 \end{bmatrix} = \begin{bmatrix} 1 & 0 \\ 0 & 1 \end{bmatrix} = I$$

$$\therefore AA^0 = I \text{ --- (1)}$$

now consider

$$A^0A = \frac{1}{2} \begin{bmatrix} 1-i & 1-i \\ -1-i & 1+i \end{bmatrix} \frac{1}{2} \begin{bmatrix} 1+i & -1+i \\ 1+i & 1-i \end{bmatrix}$$

$$= \frac{1}{4} \begin{bmatrix} 1-i & 1-i \\ -1-i & 1+i \end{bmatrix} \begin{bmatrix} 1+i & -1+i \\ 1+i & 1-i \end{bmatrix}$$

$$A^0A = \frac{1}{4} \begin{bmatrix} 4 & 0 \\ 0 & 4 \end{bmatrix} = \begin{bmatrix} 1 & 0 \\ 0 & 1 \end{bmatrix} = I$$

$$\therefore A^0A = I \text{ --- (2)}$$

From eqn (1) and (2), we have

$$AA^0 = A^0A = I$$

$\therefore A$  is unitary matrix.

we have

$$A^{-1}A^0 = \frac{1}{2} \begin{bmatrix} 1-i & 1-i \\ -1-i & 1+i \end{bmatrix}$$